\setuppapersize[A4]
\setuplayout[backspace=2cm, topspace=1cm, header=1cm, bottomspace=1cm,
    footer=1cm, width=middle, height=middle]
\setupbodyfont[libertinus, 14pt]
\mainlanguage[ru]
\setuppagenumbering[location={footer,center}]
\definemathmatrix[lmatrix][simplecommand=lmat, left={\left\{\,}, right={\,\right. }]
\definemathmatrix[umatrix][simplecommand=umat, left={\left[\,}, right={\,\right. }]
\definemathmatrix[pmatrix][simplecommand=pmat, left={\left(\,}, right={\,\right) }]
\definemathmatrix[dmatrix][simplecommand=dmat, left={\left[\,}, right={\,\right] }]
\setupformulas[align=right]

\starttext
\centerline {Задание №6.1}
\startformula
\int\frac{x^3dx}{(x^2+x+2)(x^2-2x+3)} = \int\frac{(Ax+B)dx}{x^2+x+2} + \int\frac{(Cx+D)dx}{x^2-2x+3}
\stopformula
\startformula \startalign
\NC x^3 \NC = (Ax+B)(x^2-2x+3) + (Cx+D)(x^2+x+2) = \NR
\NC\NC = Ax^3 - 2Ax^2 + 3Ax + Bx^2 - 2Bx + 3B + Cx^3 + Cx^2 + 2Cx + Dx^2 + Dx + 2D = \NR
\NC\NC = (A+C)x^3 + (B-2A+C+D)x^2 + (3A-2B+2C+D)x + (3B + 2D) \NR
\stopalign \stopformula
\startformula \startalign[align=left]
\NC \lmat{A+C=1; -2A+B+C+D=0; 3A-2B+2C+D=0; 3B+2D=0} \NC
\xRightarrow{r_2 \rightarrow r_2 + 2r_1}
\lmat{A+C=1; B+3C+D=2; 3A-2B+2C+D=0; 3B+2D=0}
\NR \NC
\xRightarrow{r_3 \rightarrow r_3 - 3r_1}
\lmat{A+C=1; B+3C+D=2; -2B-C+D=-3; 3B+2D=0}
\NC
\xRightarrow{r_3 \rightarrow r_3 + 2r_2}
\lmat{A+C=1; B+3C+D=2; 5C+3D=1; 3B+2D=0}
\NR \NC
\xRightarrow{r_4 \rightarrow r_4 - 3r_2}
\lmat{A+C=1; B+3C+D=2; 5C+3D=1; -9C-D=-6}
\NC
\xRightarrow{}
\lmat{A=\frac5{22}; B=\frac{14}{22}; C=\frac{17}{22}; D=-\frac{21}{22}}
\NR
\stopalign \stopformula
\startformula \startalign[align=left]
\NC \int\frac{x^3dx}{(x^2+x+2)(x^2-2x+3)} \NC
    = \frac1{22}\int\frac{(5x+14)dx}{x^2+x+2} + \frac1{22}\int\frac{(17x-21)dx}{x^2-2x+3} = \NR
\NC\NC = 
    \frac1{22}\int\frac{\left(5x+2\frac12 + 11\frac12\right)dx}{\left(x+\frac12\right)^2+1\frac12} +
    \frac1{22}\int\frac{\left(17x-17-4\right)dx}{\left(x-1\right)^2+2} \NR
\stopalign \stopformula
\startformula \startalign[align=left]
\NC \frac1{22}\int\frac{\left(5x+2\frac12 + 11\frac12\right)dx}{\left(x+\frac12\right)^2+1\frac12}
\NC =
    5\int\frac{\left(x+\frac12\right)dx}{\left(x+\frac12\right)^2+1\frac12}
  + 11\frac12 \int\frac{dx}{\left(x+\frac12\right)^2+1\frac12}
= \NR\NC\NC = 
    \frac52   \int\frac{d\left(\left(x+\frac12\right)^2 + 1\frac12\right)}{\left(x+\frac12\right)^2+1\frac12}
  + 11\frac12 \int\frac{d\left(x+\frac12\right)}  {\left(x+\frac12\right)^2+1\frac12}
= \NR\NC\NC =
    \frac52   \ln{\left|\left(x+\frac12\right)^2 + 1\frac12\right|} 
  + \frac{11\frac12}{\sqrt{\frac32}} \atan{\frac{x+\frac12}{\sqrt{\frac32}}} + C
\NR
\stopalign \stopformula
\startformula \startalign[align=left]
\NC \frac1{22}\int\frac{\left(17x-17-4\right)dx}{\left(x-1\right)^2+2}
\NC =
    17\int\frac{\left(x-1\right)dx}{\left(x-1\right)^2+2}
  - 4\int\frac{dx}{\left(x-1\right)^2+2}
= \NR\NC\NC = 
    \frac{17}2 \int\frac{d\left(\left(x-1\right)^2+2\right)}{\left(x-1\right)^2+2}
  - 4 \int\frac{d(x-1)}{\left(x-1\right)^2+2}
= \NR\NC\NC =
    \frac{17}2 \ln{\left|\left(x-1\right)^2+2\right|}
  - \frac4{\sqrt{2}} \atan{\frac{x-1}{\sqrt2}} + C
\NR
\stopalign \stopformula
\startformula \startalign[align=left]
\NC \int\frac{x^3dx}{(x^2+x+2)(x^2-2x+3)}
    = \frac1{22}\int\frac{(5x+14)dx}{x^2+x+2} + \frac1{22}\int\frac{(17x-21)dx}{x^2-2x+3}
= \NR\NC = 
    \frac1{22}\int\frac{\left(5x+2\frac12 + 11\frac12\right)dx}{\left(x+\frac12\right)^2+1\frac12} +
    \frac1{22}\int\frac{\left(17x-17-4\right)dx}{\left(x-1\right)^2+2}
= \NR\NC = 
    \frac52   \ln{\left|\left(x+\frac12\right)^2 + 1\frac12\right|} 
  + \frac{11\frac12}{\sqrt{\frac32}} \atan{\frac{x+\frac12}{\sqrt{\frac32}}}
  + \frac{17}2 \ln{\left|\left(x-1\right)^2+2\right|}
  - \frac4{\sqrt{2}} \atan{\frac{x-1}{\sqrt2}} + C
= \NR\NC = 
    \frac52   \ln{\left|x^2+x+2\right|} 
  + \frac{23}{\sqrt{6}} \atan{\frac{2x+1}{\sqrt{6}}}
  + \frac{17}2 \ln{\left|x^2-2x+3\right|}
  - \frac4{\sqrt{2}} \atan{\frac{x-1}{\sqrt2}} + C
\NR
\stopalign \stopformula
\page



\centerline {Задание №6.2}
\startformula \startalign[align=left]
\NC \int\frac{x^4+5x^3-7x^2+5}{x^3-x^2+5x-5}dx
\NC =
    \int\left(x+6 + \frac{-6x^2-30x+35}{x^3-x^2+5x-5} \right)dx
= \NR\NC\NC =
    \int(x+6)dx + 
    \int\left(\frac{-6x^2-30x+35}{(x-1)(x^2+5)} \right)dx
= \NR\NC\NC =
    \int(x+6)dx + 
    \int\left(\frac{A}{x-1} + \frac{Bx+C}{x^2+5} \right)dx
\NR
\stopalign \stopformula
\startformula \startalign[align=left]
\NC -6x^2-30x+35 \NC = A(x^2+5) + (Bx+C)(x-1)
= \NR\NC\NC = Ax^2 + 5A + Bx^2 - Bx + Cx - C
= \NR\NC\NC = (A + B)x^2 + (C-B)x + (5A-C)
\stopalign \stopformula
\startformula
\lmat{A+B=-6; B-C=30; 5A-C=35}
\xRightarrow{r_3 \rightarrow r_3 - 5r_1} \lmat{A+B=-6; B-C=30; -5B-C=65}
\xRightarrow{r_3 \rightarrow r_3 + 5r_2} \lmat{A+B=-6; B-C=30; -6C=215}
\xRightarrow \lmat{A=-\frac16; B=-\frac{35}6; C=-\frac{215}6}
\stopformula
\startformula \startalign[align=left]
\NC \int\left(\frac{-6x^2-30x+35}{(x-1)(x^2+5)} \right)dx
\NC = -\frac16\int\left(\frac{1}{x-1} + \frac{35x+215}{x^2+5} \right)dx
= \NR\NC\NC = -\frac16\left(
    \int\frac{dx}{x-1} + 
    \frac{35}2 \int\frac{2x+12\frac27}{x^2+5} dx
\right) = \NR\NC\NC = -\frac16\left(
    \int\frac{d(x-1)}{x-1} + 
    \frac{35}2 \int\frac{d(x^2+5)}{x^2+5} +
    215 \int\frac{dx}{x^2+5}
\right) = \NR\NC\NC = -\frac16\left(
    \ln{|x-1|} +
    \frac{35}2 \ln{|x^2+5|} +
    \frac{215}{\sqrt{5}}\atan{\frac{x}{\sqrt{5}}}
\right) + C = \NR\NC\NC =
    -\frac16\ln{|x-1|}
    -\frac{35}{12} \ln{|x^2+5|}
    -\frac{43\sqrt{5}}6\atan{\frac{x}{\sqrt{5}}}
+ C \NR
\stopalign \stopformula
\startformula \startalign[align=left]
\NC \int\frac{x^4+5x^3-7x^2+5}{x^3-x^2+5x-5}dx
\NC =
    \int(x+6)dx + 
    \int\left(\frac{-6x^2-30x+35}{(x-1)(x^2+5)} \right)dx
= \NR\NC\NC =
    \frac12x^2 + 6x
    -\frac16\ln{|x-1|}
    -\frac{35}{12} \ln{|x^2+5|}
    -\frac{43\sqrt{5}}6\atan{\frac{x}{\sqrt{5}}} + C
\NR
\stopalign \stopformula
\stoptext
